Removed last admits from changing Decidable definition

theories/L6_PCPS/identifiers.v
@@ -843,7 +843,7 @@ Proof.
   apply occurs_free_ctx_mut.
 Qed.
 
-Corollary occurs_free_fundefs_ctx :
+Corollary occurs_free_fundefs_ctx_c :
   forall B e e', Same_set _ (occurs_free e) (occurs_free e') ->
                  Same_set _ (occurs_free_fundefs (B <[ e ]>))
                           (occurs_free_fundefs (B <[ e' ]>)).
@@ -3796,74 +3796,116 @@ Qed.
 
 Local Hint Constructors bound_var_ctx bound_var_fundefs_ctx.
 
-(* Lemma bound_var_ctx_dec_mut : *)
-(*   (forall c, Decidable (bound_var_ctx c)) /\ *)
-(*   (forall Bc, Decidable (bound_var_fundefs_ctx Bc)). *)
-(* Proof. *)
-(*   exp_fundefs_ctx_induction IHc IHf; split; intro x; try (inv IHc; specialize (Dec x); inv Dec; auto); *)
-(*   try (inv IHf; specialize (Dec x); inv Dec; auto). *)
-(*   - right; intro; inv H. *)
-(*   - destruct (var_dec v x); subst; auto. *)
-(*     right; intro Hbv; inv Hbv; auto. *)
-(*   - destruct (var_dec v x); subst; auto. *)
-(*     right; intro Hbv; inv Hbv; auto. *)
-(*   - destruct (var_dec v x); subst; auto. *)
-(*     right; intro Hbv; inv Hbv; auto. *)
-(*   - destruct (bound_var_dec (Ecase v l)). *)
-(*     specialize (Dec x). *)
-(*     inv Dec; auto. *)
-(*     left. *)
-(*     inv H0. *)
-(*     eapply Bound_Case2_c; eauto. *)
-(*     destruct (bound_var_dec (Ecase v l0)). *)
-(*     specialize (Dec x). *)
-(*     inv Dec; auto. *)
-(*     left. *)
-(*     inv H1. *)
-(*     eapply Bound_Case3_c; eauto. *)
-(*     right. *)
-(*     intro. inv H2; auto. *)
-(*     apply H0; eauto. *)
-(*     apply H1; eauto. *)
-(*   - destruct (bound_var_fundefs_dec f4). *)
-(*     specialize (Dec x). *)
-(*     inv Dec; auto. *)
-(*     right. intro. *)
-(*     inv H1; auto. *)
-(*   - destruct (bound_var_dec e). *)
-(*     specialize (Dec x). *)
-(*     inv Dec; auto. *)
-(*     right. intro. *)
-(*     inv H1; auto.  *)
-(*   - destruct (bound_var_fundefs_dec f6). *)
-(*     specialize (Dec x). *)
-(*     inv Dec; auto. *)
-(*     destruct (var_dec v x); subst; auto. *)
-(*     destruct (in_dec var_dec x l); auto. *)
-(*     right. *)
-(*     intro. inv H1; auto. *)
-(*   - destruct (bound_var_dec e). *)
-(*     specialize (Dec x). *)
-(*     inv Dec; auto. *)
-(*     destruct (var_dec v x); subst; auto. *)
-(*     destruct (in_dec var_dec x l); auto. *)
-(*     right. *)
-(*     intro. inv H1; auto. *)
-(* Qed. *)
-
 Theorem bound_var_ctx_dec :
   forall c, Decidable (bound_var_ctx c).
 Proof.
-Admitted. (*   apply bound_var_ctx_dec_mut. *)
-(* Qed. *)
-
+  eapply ctx_exp_mut' with (P0 := fun B => Decidable (bound_var_fundefs_ctx B));
+  constructor; intros x.
+  - right; intros Hc; inv Hc.
+  - destruct (var_dec v x); subst; auto.
+    destruct H as [Dec]. destruct (Dec x).
+    now left; eauto.
+    now right; intro Hbv; inv Hbv; auto.
+  - destruct (var_dec v x); subst; auto.
+    destruct H as [Dec]. destruct (Dec x).
+    now left; eauto.
+    now right; intro Hbv; inv Hbv; auto.
+  - destruct (var_dec v x); subst; auto.
+    destruct H as [Dec]. destruct (Dec x).
+    now left; eauto.
+    now right; intro Hbv; inv Hbv; auto.
+  - destruct (bound_var_dec (Ecase v l)) as [Decl].
+    destruct (Decl x) as [Hb | Hnb].
+    left. now inv Hb; eauto.
+    destruct (bound_var_dec (Ecase v l0)) as [Decl'].
+    destruct (Decl' x) as [Hb' | Hnb'].
+    left. now inv Hb'; eauto.
+    destruct H as [Dec]. destruct (Dec x).
+    left; eauto.
+    right. intros Hc. inv Hc; auto.
+    now eapply Hnb; eauto.
+    now eapply Hnb'; eauto.
+  - destruct (bound_var_fundefs_dec f) as [Decf].
+    destruct (Decf x) as [Hb | Hnb]; eauto.
+    destruct H as [Dec]. destruct (Dec x).
+    left; eauto.
+    right. intros Hc. inv Hc; auto.
+  - destruct (bound_var_dec e) as [Dece].
+    destruct (Dece x) as [Hb | Hnb]; eauto.
+    destruct H as [Dec]. destruct (Dec x).
+    left; eauto.
+    right. intros Hc. inv Hc; auto.    
+  - destruct (bound_var_fundefs_dec f) as [Decf].
+    destruct (Decf x) as [Hb | Hnb]; eauto.
+    destruct H as [Dec]. destruct (Dec x).
+    left; eauto.
+    destruct (var_dec v x); subst; auto.
+    destruct (in_dec var_dec x l); auto. 
+    right. intros Hc. inv Hc; auto.
+  - destruct (bound_var_dec e) as [Dece].
+    destruct (Dece x) as [Hb | Hnb]; eauto.
+    destruct H as [Dec]. destruct (Dec x).
+    left; eauto.
+    destruct (var_dec v x); subst; auto.
+    destruct (in_dec var_dec x l); auto. 
+    right. intros Hc. inv Hc; auto.
+Qed.
 
 Theorem bound_var_fundefs_ctx_dec :
   forall Bc, Decidable (bound_var_fundefs_ctx Bc).
 Proof.
-Admitted.
-(* apply bound_var_ctx_dec_mut. *)
-(* Qed. *)
+  eapply ctx_fundefs_mut' with (P := fun e => Decidable (bound_var_ctx e));
+  constructor; intros x.
+  - right; intros Hc; inv Hc.
+  - destruct (var_dec v x); subst; auto.
+    destruct H as [Dec]. destruct (Dec x).
+    now left; eauto.
+    now right; intro Hbv; inv Hbv; auto.
+  - destruct (var_dec v x); subst; auto.
+    destruct H as [Dec]. destruct (Dec x).
+    now left; eauto.
+    now right; intro Hbv; inv Hbv; auto.
+  - destruct (var_dec v x); subst; auto.
+    destruct H as [Dec]. destruct (Dec x).
+    now left; eauto.
+    now right; intro Hbv; inv Hbv; auto.
+  - destruct (bound_var_dec (Ecase v l)) as [Decl].
+    destruct (Decl x) as [Hb | Hnb].
+    left. now inv Hb; eauto.
+    destruct (bound_var_dec (Ecase v l0)) as [Decl'].
+    destruct (Decl' x) as [Hb' | Hnb'].
+    left. now inv Hb'; eauto.
+    destruct H as [Dec]. destruct (Dec x).
+    left; eauto.
+    right. intros Hc. inv Hc; auto.
+    now eapply Hnb; eauto.
+    now eapply Hnb'; eauto.
+  - destruct (bound_var_fundefs_dec f) as [Decf].
+    destruct (Decf x) as [Hb | Hnb]; eauto.
+    destruct H as [Dec]. destruct (Dec x).
+    left; eauto.
+    right. intros Hc. inv Hc; auto.
+  - destruct (bound_var_dec e) as [Dece].
+    destruct (Dece x) as [Hb | Hnb]; eauto.
+    destruct H as [Dec]. destruct (Dec x).
+    left; eauto.
+    right. intros Hc. inv Hc; auto.    
+  - destruct (bound_var_fundefs_dec f) as [Decf].
+    destruct (Decf x) as [Hb | Hnb]; eauto.
+    destruct H as [Dec]. destruct (Dec x).
+    left; eauto.
+    destruct (var_dec v x); subst; auto.
+    destruct (in_dec var_dec x l); auto. 
+    right. intros Hc. inv Hc; auto.
+  - destruct (bound_var_dec e) as [Dece].
+    destruct (Dece x) as [Hb | Hnb]; eauto.
+    destruct H as [Dec]. destruct (Dec x).
+    left; eauto.
+    destruct (var_dec v x); subst; auto.
+    destruct (in_dec var_dec x l); auto. 
+    right. intros Hc. inv Hc; auto.
+Qed.
+
 
 Fixpoint names_in_fundefs_ctx B:=
   match B with
@@ -4083,3 +4125,529 @@ Theorem decidable_ub_fundefs:
 Proof.
   intros. apply decidable_ub_mut.
 Qed.
+
+(** * Free variables for expression and function contexts *)
+
+(** set of free variables for an applicative context *)
+Inductive occurs_free_ctx : exp_ctx -> Ensemble var :=
+| Free_ctx_Econstr1 :
+    forall y x t ys e,
+      List.In y ys ->
+      occurs_free_ctx (Econstr_c x t ys e) y
+| Free_ctx_Econstr2 :
+    forall y x t ys e,
+      ~ x = y ->
+      occurs_free_ctx e y ->
+      occurs_free_ctx (Econstr_c x t ys e) y
+| Free_ctx_Ecase1 :
+    forall x cl1 c e cl2, 
+      occurs_free_ctx (Ecase_c x cl1 c e cl2) x
+| Free_ctx_Ecase2 :  
+    forall y x cl1 c e cl2,
+      occurs_free_ctx e y ->
+      occurs_free_ctx (Ecase_c x cl1 c e cl2) y
+| Free_ctx_Ecase3 :  
+    forall y x cl1 c e cl2,
+      occurs_free (Ecase x cl1) y ->
+      occurs_free_ctx (Ecase_c x cl1 c e cl2) y
+| Free_ctx_Ecase4 :  
+    forall y x cl1 c e cl2,
+      occurs_free (Ecase x cl2) y ->
+      occurs_free_ctx (Ecase_c x cl1 c e cl2) y
+| Free_ctx_Eproj1 :
+    forall y x tau n e,
+      occurs_free_ctx (Eproj_c x tau n y e) y
+| Free_ctx_Eproj2 :
+    forall y x tau n y' e,
+      x <> y ->
+      occurs_free_ctx e y ->
+      occurs_free_ctx (Eproj_c x tau n y' e) y
+| Free_ctx_Efun11 :
+    forall y defs e,
+      ~ (name_in_fundefs defs y) -> 
+      occurs_free_ctx e y ->
+      occurs_free_ctx (Efun1_c defs e) y
+| Free_ctx_Efun21 :
+    forall y defs e,
+      ~ (names_in_fundefs_ctx defs y) -> 
+      occurs_free e y ->
+      occurs_free_ctx (Efun2_c defs e) y                             
+| Free_ctx_Efun12 :
+    forall y defs e, 
+      occurs_free_fundefs defs y ->
+      occurs_free_ctx (Efun1_c defs e) y
+| Free_ctx_Efun22 :
+    forall y defs e, 
+      occurs_free_fundefs_ctx defs y ->
+      occurs_free_ctx (Efun2_c defs e) y
+| Free_ctx_Eprim1 :
+    forall y x p ys e,
+      List.In y ys ->
+      occurs_free_ctx (Eprim_c x p ys e) y
+| Free_ctx_Eprim2 :
+    forall y x p ys e,
+      x <> y ->
+      occurs_free_ctx e y ->
+      occurs_free_ctx (Eprim_c x p ys e) y
+with occurs_free_fundefs_ctx : fundefs_ctx -> Ensemble var :=
+      | Free_ctx_Fcons11 :
+          forall x f tau ys e defs,  
+            x <> f ->
+            ~ (List.In x ys) ->
+            ~ (name_in_fundefs defs x) ->
+            occurs_free_ctx e x ->
+            occurs_free_fundefs_ctx (Fcons1_c f tau ys e defs) x
+      | Free_ctx_Fcons12 :
+          forall x f tau ys e defs,
+            occurs_free_fundefs defs x ->
+            x <> f ->
+            occurs_free_fundefs_ctx (Fcons1_c f tau ys e defs) x
+      | Free_ctx_Fcons21 :
+          forall x f tau ys e defs,  
+            x <> f ->
+            ~ (List.In x ys) ->
+            ~ (names_in_fundefs_ctx defs x) ->
+            occurs_free e x ->
+            occurs_free_fundefs_ctx (Fcons2_c f tau ys e defs) x
+      | Free_ctx_Fcons22 :
+          forall x f tau ys e defs,
+            occurs_free_fundefs_ctx defs x ->
+            x <> f ->
+            occurs_free_fundefs_ctx (Fcons2_c f tau ys e defs) x.
+
+Hint Constructors occurs_free_ctx occurs_free_fundefs.
+
+Lemma occurs_free_Econstr_c x t ys e :
+  Same_set var (occurs_free_ctx (Econstr_c x t ys e))
+           (Union _ (FromList ys) (Setminus var (occurs_free_ctx e) (Singleton var x))).
+Proof.
+  split; intros x' H; inv H; eauto.
+  right. constructor; eauto. intros H. inv H; eauto.
+  inv H0.  constructor 2; eauto. intros Hc. subst. eauto.
+Qed.
+
+Lemma occurs_free_Eprim_c x f ys e :
+  Same_set var (occurs_free_ctx (Eprim_c x f ys e))
+           (Union _ (FromList ys) (Setminus var (occurs_free_ctx e) (Singleton var x))).
+Proof.
+  split; intros x' H; inv H; eauto.
+  right. constructor; eauto. intros H. inv H; eauto.
+  inv H0. eapply Free_ctx_Eprim2; eauto. intros Hc. subst. eauto.
+Qed.
+
+Lemma occurs_free_Eproj_c x tag n y e :
+  Same_set var (occurs_free_ctx (Eproj_c x tag n y e))
+           (Union _ (Singleton var y) (Setminus var (occurs_free_ctx e) (Singleton var x))).
+Proof.
+  split; intros x' H; inv H; eauto. 
+  right. constructor; eauto. intros H. inv H; eauto.
+  inv H0. eauto.
+  inv H0. constructor; eauto.
+  intros Hc. subst. eauto.
+Qed.
+
+Lemma occurs_free_Efun1_c B e :
+  Same_set var (occurs_free_ctx (Efun1_c B e))
+           (Union _ (occurs_free_fundefs B)
+                  (Setminus _ (occurs_free_ctx e) (name_in_fundefs B))).
+Proof.
+  split; intros x' H; inv H; eauto.
+  right; eauto. constructor; eauto.
+  inv H0. eauto. 
+Qed.
+
+Lemma occurs_free_Efun2_c B e :
+  Same_set var (occurs_free_ctx (Efun2_c B e))
+           (Union _ (occurs_free_fundefs_ctx B)
+                  (Setminus _ (occurs_free e) (names_in_fundefs_ctx B))).
+Proof.
+  split; intros x' H; inv H; eauto.
+  right; eauto. constructor; eauto.
+  inv H0. eauto. 
+Qed.
+
+
+Lemma occurs_free_Ecase_c x cl1 cl2 c e :
+  Same_set var (occurs_free_ctx (Ecase_c x cl1 c e cl2))
+           (Union _ (Singleton _ x)
+                  (Union _ (occurs_free_ctx e)
+                         (Union _ (occurs_free (Ecase x cl1)) (occurs_free (Ecase x cl2))))).
+Proof.
+  split; intros x' H; inv H; eauto.
+  inv H0; eauto. inv H0; eauto.
+  inv H; eauto.
+Qed.
+
+
+Lemma occurs_free_fundefs_Fcons1_c f t xs e B :
+  Same_set var (occurs_free_fundefs_ctx (Fcons1_c f t xs e B))
+           (Union var (Setminus var (occurs_free_ctx e)
+                                (Union var (Singleton var f)
+                                       (Union var (FromList xs)
+                                              (name_in_fundefs B))))
+                  (Setminus var (occurs_free_fundefs B) (Singleton var f))).
+Proof.
+  split; intros x H; inv H.
+  - left. constructor; eauto. intros Hin. inv Hin; eauto.
+    inv H. congruence. inv H; eauto.
+  - right. constructor; eauto. intros H. inv H. congruence.
+  - inv H0. constructor; eauto. 
+    intros Hc. subst. eauto.
+  - inv H0. constructor 2; eauto. intros Hc; subst; eauto.
+Qed.
+
+Lemma occurs_free_fundefs_Fcons2_c f t xs e B :
+  Same_set var (occurs_free_fundefs_ctx (Fcons2_c f t xs e B))
+           (Union var (Setminus var (occurs_free e)
+                                (Union var (Singleton var f)
+                                       (Union var (FromList xs)
+                                              (names_in_fundefs_ctx B))))
+                  (Setminus var (occurs_free_fundefs_ctx B) (Singleton var f))).
+Proof.
+  split; intros x H; inv H.
+  - left. constructor; eauto. intros Hin. inv Hin; eauto.
+    inv H. congruence. inv H; eauto.
+  - right. constructor; eauto. intros H. inv H. congruence.
+  - inv H0. constructor; eauto. 
+    intros Hc. subst. eauto.
+  - inv H0.
+    constructor 4;  eauto.
+    intros Hc; subst; eauto.
+Qed.
+
+Lemma occurs_free_Hole_c:
+  Same_set var (occurs_free_ctx Hole_c)
+           (Empty_set var).
+Proof.
+  split; intros x H; inv H.
+Qed.
+
+
+Ltac normalize_occurs_free_ctx :=
+  match goal with
+    | [|- context[occurs_free_ctx (Econstr_c _ _ _ _)]] =>
+      rewrite occurs_free_Econstr_c
+    | [|- context[occurs_free_ctx (Eproj_c _ _ _ _ _)]] =>
+      rewrite occurs_free_Eproj_c
+    | [|- context[occurs_free_ctx (Ecase_c _ _ _ _ _ )]] =>
+      rewrite occurs_free_Ecase_c
+    | [|- context[occurs_free_ctx (Efun1_c _ _)]] =>
+      rewrite occurs_free_Efun1_c
+    | [|- context[occurs_free_ctx (Efun2_c _ _)]] =>
+      rewrite occurs_free_Efun2_c
+    | [|- context[occurs_free_ctx (Eprim_c _ _ _ _)]] =>
+      rewrite occurs_free_Eprim_c
+    | [|- context[occurs_free_fundefs_ctx (Fcons1_c _ _ _ _ _)]] =>
+      rewrite occurs_free_fundefs_Fcons1_c
+    | [|- context[occurs_free_fundefs_ctx (Fcons2_c _ _ _ _ _)]] =>
+      rewrite occurs_free_fundefs_Fcons2_c
+    | [|- context[occurs_free_ctx (Hole_c)]] =>
+      rewrite occurs_free_Hole_c
+  end.
+
+Ltac normalize_occurs_free_ctx_in_ctx :=
+  match goal with
+    | [ H : context[occurs_free_ctx (Econstr_c _ _ _ _)] |- _ ] =>
+      rewrite occurs_free_Econstr_c
+    | [ H : context[occurs_free_ctx (Eproj_c _ _ _ _ _)] |- _ ] =>
+      rewrite occurs_free_Eproj_c
+    | [ H : context[occurs_free_ctx (Ecase_c _ _ _ _ _ )] |- _ ] =>
+      rewrite occurs_free_Ecase_c
+    | [ H : context[occurs_free_ctx (Efun1_c _ _)] |- _ ] =>
+      rewrite occurs_free_Efun1_c
+    | [ H : context[occurs_free_ctx (Efun2_c _ _)] |- _ ] =>
+      rewrite occurs_free_Efun2_c
+    | [ H : context[occurs_free_ctx (Eprim_c _ _ _ _)] |- _ ] =>
+      rewrite occurs_free_Eprim_c
+    | [ H : context[occurs_free_fundefs_ctx (Fcons1_c _ _ _ _ _)] |- _ ] =>
+      rewrite occurs_free_fundefs_Fcons1_c
+    | [ H : context[occurs_free_fundefs_ctx (Fcons2_c _ _ _ _ _)] |- _ ] =>
+      rewrite occurs_free_fundefs_Fcons2_c
+    | [ H : context[occurs_free_ctx (Hole_c)] |- _ ] =>
+      rewrite occurs_free_Hole_c
+  end.
+
+  Definition closed_ctx :=
+    fun c => Empty_set var <--> occurs_free_ctx c.
+  
+  Definition closed_fundefs_ctx :=
+    fun cf => Empty_set var <--> occurs_free_fundefs_ctx cf.
+
+  Theorem fun_names_not_free_in_fundefs_ctx :
+    forall x f7,
+      names_in_fundefs_ctx f7 x
+      -> ~ occurs_free_fundefs_ctx f7 x.
+  Proof.
+    induction f7; intros; intro.
+    inv H; inv H0; auto.
+    inv H1; auto.
+    inv H1; auto.
+    revert H7.
+    apply fun_names_not_free_in_fundefs.
+    auto.
+    inv H; inv H0; auto.
+    inv H1; auto.
+    inv H1; auto.
+    revert H7.
+    apply IHf7; auto.
+  Qed.
+
+  Lemma occurs_free_included_ctx_mut:
+    forall e,
+      (forall c,
+         Included _ (occurs_free_ctx c) (occurs_free (c|[e]|))) /\
+      (forall fc,
+         Included _ (occurs_free_fundefs_ctx fc) (occurs_free_fundefs (fc <[ e ]>))).
+  Proof.
+    intro e; exp_fundefs_ctx_induction IHc IHf; intros; repeat normalize_occurs_free_ctx; simpl; repeat normalize_occurs_free; eauto with Ensembles_DB.
+    rewrite <- name_in_fundefs_ctx_ctx.
+    eauto with Ensembles_DB.
+    rewrite <- name_in_fundefs_ctx_ctx.
+    eauto with Ensembles_DB.
+  Qed.
+
+  Theorem occurs_free_included_ctx:
+    forall e,
+      (forall c,
+         Included _ (occurs_free_ctx c) (occurs_free (c|[e]|))).
+  Proof.
+    intros; apply occurs_free_included_ctx_mut.
+  Qed.
+
+  Theorem occurs_free_included_fundefs_ctx:
+    forall e,
+      (forall fc,
+         Included _ (occurs_free_fundefs_ctx fc) (occurs_free_fundefs (fc <[ e ]>))).
+  Proof.
+    intros; apply occurs_free_included_ctx_mut.
+  Qed.
+
+
+  Theorem Decidable_occurs_free_ctx :
+    (forall c,
+       Decidable (occurs_free_ctx c)).
+  Proof.
+    eapply ctx_exp_mut' with (P0 := fun B => Decidable (occurs_free_fundefs_ctx B));
+    constructor; intros x; try (inv IHc; specialize (Dec x)); try (inv IHf; specialize (Dec x)).
+    - right; auto.
+      intro. inv H.
+    - assert (Hl := Decidable_FromList l).
+      destruct Hl as [Decl].
+      specialize (Decl x).
+      inv Decl.
+      left; auto.
+      destruct (var_dec  v x).
+      subst.
+      right.
+      intro Hc.
+      inv Hc. auto.
+      now apply H6; auto.
+      destruct H as [Dec].
+      destruct (Dec x).
+      left; auto.
+      right.
+      intro Hc. inv Hc; auto.
+    - destruct (var_dec x v0).
+      now subst; left; auto.
+      destruct (var_dec v x).
+      subst.
+      now right; intro Hc; inv Hc; auto.
+      destruct H as [Dec]; destruct (Dec x).
+      left; auto.
+      right; intro Hc.
+      inv Hc; auto.
+    - assert (Hl := Decidable_FromList l).
+      inv Hl.
+      destruct (Dec x).
+       left; auto.
+      destruct (var_dec  v x).
+      subst.
+      right.
+      intro.
+      inv H0. auto.
+      apply H6; auto.
+      destruct H as [Dece]; destruct (Dece x).
+      now left; auto.
+      right.
+      intro Hc. inv Hc; auto.
+    - assert (Hl := Decidable_occurs_free (Ecase v l)).
+      assert (Hl0 := Decidable_occurs_free (Ecase v l0)).
+      destruct Hl as [Decl].
+      destruct Hl0 as [Decl0].
+      destruct H as [Dec].
+      destruct (Decl x).
+      left. now apply Free_ctx_Ecase3; auto.
+      destruct (Decl0 x).
+      left. now apply Free_ctx_Ecase4; auto.
+      destruct (Dec x). 
+      left. constructor; auto.
+      right. intro Hc.
+      inv Hc; auto.
+    - assert (Hf4 := Decidable_occurs_free_fundefs f).
+      destruct Hf4 as [Decf]. destruct (Decf x). 
+      now left; auto.
+      assert (Hf4n := Decidable_name_in_fundefs f).
+      destruct Hf4n as [Decf0]. destruct (Decf0 x).
+      right.
+      intro Hc.
+      inv Hc; auto.
+      destruct H as [Dec]. destruct (Dec x).
+      left; auto.
+      right; intro Hc. inv Hc; auto.
+    - assert (He := Decidable_occurs_free e).
+      destruct H as [Decf]. destruct He as [Dece].
+      destruct (Decf x); eauto.
+      assert (Hf5 := Decidable_name_in_fundefs_ctx f).
+      inv Hf5. destruct (Dec x); eauto.
+      right. intros Hc; inv Hc; try contradiction.
+      destruct (Dece x); eauto.
+      right. intros Hc; inv Hc; try contradiction.
+    - destruct (var_dec x v).
+      subst. right.
+      now intros Hc; inv Hc; auto.
+      assert (Hf6 := Decidable_name_in_fundefs f).
+      inv Hf6. destruct (Dec x).
+      right. intros Hc. inv Hc; try contradiction.
+      now apply fun_names_not_free_in_fundefs in H6; auto.
+      assert (He := Decidable_occurs_free_fundefs f).
+      destruct He as [Dece]. destruct (Dece x).
+      now left; constructor 2; auto.
+      destruct H as [Dece']. destruct (Dece' x); eauto.
+      assert (Hl := Decidable_FromList l).
+      destruct Hl as [Decl]. destruct (Decl x).
+      now right; intros Hc; inv Hc; auto.
+      now left; constructor; auto.
+      right. intros Hc. inv Hc; auto.
+    - destruct (var_dec x v).
+      right.
+      intros Hc. subst. inv Hc; auto.
+      assert (Hf := Decidable_name_in_fundefs_ctx f).
+      destruct Hf as [Decf]. destruct (Decf x).
+      right. intros Hc. inv Hc.
+      contradiction.
+      now apply fun_names_not_free_in_fundefs_ctx in H6; auto.
+      destruct H as [Dec]. destruct (Dec x).
+      left; constructor 4; auto.
+      assert (Hl := Decidable_FromList l).
+      inv Hl. destruct (Dec0 x).
+      right; intros Hc; inv Hc; auto.
+      assert (He :=  Decidable_occurs_free e).
+      destruct He as [Dece].
+      destruct (Dece x). now left; constructor; auto.
+      now right; intros Hc; inv Hc; auto.
+  Qed.
+
+  
+
+  Theorem Decidable_occurs_free_fundefs_ctx :
+    (forall fc, Decidable (occurs_free_fundefs_ctx fc)).
+  Proof.
+    eapply ctx_fundefs_mut' with (P := fun e => Decidable (occurs_free_ctx e));
+    constructor; intros x; try (inv IHc; specialize (Dec x)); try (inv IHf; specialize (Dec x)).
+    - right; auto.
+      intro. inv H.
+    - assert (Hl := Decidable_FromList l).
+      destruct Hl as [Decl].
+      specialize (Decl x).
+      inv Decl.
+      left; auto.
+      destruct (var_dec  v x).
+      subst.
+      right.
+      intro Hc.
+      inv Hc. auto.
+      now apply H6; auto.
+      destruct H as [Dec].
+      destruct (Dec x).
+      left; auto.
+      right.
+      intro Hc. inv Hc; auto.
+    - destruct (var_dec x v0).
+      now subst; left; auto.
+      destruct (var_dec v x).
+      subst.
+      now right; intro Hc; inv Hc; auto.
+      destruct H as [Dec]; destruct (Dec x).
+      left; auto.
+      right; intro Hc.
+      inv Hc; auto.
+    - assert (Hl := Decidable_FromList l).
+      inv Hl.
+      destruct (Dec x).
+       left; auto.
+      destruct (var_dec  v x).
+      subst.
+      right.
+      intro.
+      inv H0. auto.
+      apply H6; auto.
+      destruct H as [Dece]; destruct (Dece x).
+      now left; auto.
+      right.
+      intro Hc. inv Hc; auto.
+    - assert (Hl := Decidable_occurs_free (Ecase v l)).
+      assert (Hl0 := Decidable_occurs_free (Ecase v l0)).
+      destruct Hl as [Decl].
+      destruct Hl0 as [Decl0].
+      destruct H as [Dec].
+      destruct (Decl x).
+      left. now apply Free_ctx_Ecase3; auto.
+      destruct (Decl0 x).
+      left. now apply Free_ctx_Ecase4; auto.
+      destruct (Dec x). 
+      left. constructor; auto.
+      right. intro Hc.
+      inv Hc; auto.
+    - assert (Hf4 := Decidable_occurs_free_fundefs f).
+      destruct Hf4 as [Decf]. destruct (Decf x). 
+      now left; auto.
+      assert (Hf4n := Decidable_name_in_fundefs f).
+      destruct Hf4n as [Decf0]. destruct (Decf0 x).
+      right.
+      intro Hc.
+      inv Hc; auto.
+      destruct H as [Dec]. destruct (Dec x).
+      left; auto.
+      right; intro Hc. inv Hc; auto.
+    - assert (He := Decidable_occurs_free e).
+      destruct H as [Decf]. destruct He as [Dece].
+      destruct (Decf x); eauto.
+      assert (Hf5 := Decidable_name_in_fundefs_ctx f).
+      inv Hf5. destruct (Dec x); eauto.
+      right. intros Hc; inv Hc; try contradiction.
+      destruct (Dece x); eauto.
+      right. intros Hc; inv Hc; try contradiction.
+    - destruct (var_dec x v).
+      subst. right.
+      now intros Hc; inv Hc; auto.
+      assert (Hf6 := Decidable_name_in_fundefs f).
+      inv Hf6. destruct (Dec x).
+      right. intros Hc. inv Hc; try contradiction.
+      now apply fun_names_not_free_in_fundefs in H6; auto.
+      assert (He := Decidable_occurs_free_fundefs f).
+      destruct He as [Dece]. destruct (Dece x).
+      now left; constructor 2; auto.
+      destruct H as [Dece']. destruct (Dece' x); eauto.
+      assert (Hl := Decidable_FromList l).
+      destruct Hl as [Decl]. destruct (Decl x).
+      now right; intros Hc; inv Hc; auto.
+      now left; constructor; auto.
+      right. intros Hc. inv Hc; auto.
+    - destruct (var_dec x v).
+      right.
+      intros Hc. subst. inv Hc; auto.
+      assert (Hf := Decidable_name_in_fundefs_ctx f).
+      destruct Hf as [Decf]. destruct (Decf x).
+      right. intros Hc. inv Hc.
+      contradiction.
+      now apply fun_names_not_free_in_fundefs_ctx in H6; auto.
+      destruct H as [Dec]. destruct (Dec x).
+      left; constructor 4; auto.
+      assert (Hl := Decidable_FromList l).
+      inv Hl. destruct (Dec0 x).
+      right; intros Hc; inv Hc; auto.
+      assert (He :=  Decidable_occurs_free e).
+      destruct He as [Dece].
+      destruct (Dece x). now left; constructor; auto.
+      now right; intros Hc; inv Hc; auto.
+  Qed.
